0512 Prooved preservation in Nameless.v

plc/TyAndTm.sig
@@ -1,0 +1,12 @@
+ty : Type
+tm : Type
+
+TyArrow : ty -> ty -> ty
+TyForall : (bind ty in ty) -> ty
+TyUnit : ty
+
+TmApp : tm -> tm -> tm
+TmTApp : tm -> ty -> tm
+TmAbs : ty -> (bind tm in tm) -> tm
+TmTAbs : (bind ty in tm) -> tm
+TmUnit : tm
